\subsubsection{Stirling Number of the First Kind}
$S_1(n, k)$ counts the number of permutations of $n$ elements with $k$ disjoint cycles.
\begin{itemize}
  \item
    $S_1(n, k) = (n - 1) \cdot S_1(n - 1, k) + S_1(n - 1, k - 1)$
  \item
    $S_1(n, i) = [x^i] \left(\prod _ {i=0} ^ {n-1} (x + i)\right)$,
    use D\&Q and taylor shift.
  \item
    \(
    S_1(i, k) = \frac{i!}{k!} \left[x^i\right] 
    \left(\sum _ {j \ge 1} \frac{x^j}{j}\right)^k
    \)
\end{itemize}

\subsubsection{Stirling Number of the Second Kind}
$S_2(n, k)$ counts the number of ways to partition a set of $n$ elements into $k$ nonempty sets.
\begin{itemize}
  \item $S_2(n, k) = S_2(n - 1, k - 1) + k \cdot S_2(n - 1, k)$
  \item
    \(
    S_2(n, k) = \sum_{i = 0}^k \binom{k}{i}i^n (-1)^{k - i} = \sum_{i = 0}^k \frac{(-1)^i}{i!} \cdot \frac{(k - i)^n}{(k - i)!}
    \)
  \item
    \(
    S_2(i, k) = \frac{i!}{k!} [x^i] \left(e^x - 1\right)^k
    \)
\end{itemize}

\subsubsection{Derivatives/Integrals}
Integration by parts:
\(\int_a^bf(x)g(x)dx = [F(x)g(x)]_a^b-\int_a^bF(x)g'(x)dx\)
{
  \setlength{\tabcolsep}{1pt}
  \setlength{\columnsep}{0pt}

  \noindent
  \begin{tabular}{|*{20}{>{$\displaystyle}c<{$}|}}
    \frac{d}{dx}\sin^{-1} x = \frac{1}{\sqrt{1-x^2}}
    &
    \frac{d}{dx}\cos^{-1} x = -\frac{1}{\sqrt{1-x^2}}
    &
    \frac{d}{dx}\tan^{-1} x = \frac{1}{1+x^2}
    \\
    \frac{d}{dx}\tan x = 1+\tan^2 x
    &
    \int\tan ax = -\frac{\ln|\cos ax|}{a}
    &
    % \int x\sin ax = \frac{\sin ax-ax \cos ax}{a^2}
    % &
    \\
    \int e^{-x^2} = \frac{\sqrt \pi}{2} \text{erf}(x)
    &
    \int xe^{ax} dx = \frac{e^{ax}}{a^2}(ax-1)
    \\
  \end{tabular}
  
  \(
    \displaystyle
    \int \sqrt{a^2 + x^2} = \frac{1}{2} \left(x\sqrt{a^2+x^2} + a^2 \operatorname{asinh}(x/a) \right)
  \)
}

\subsubsection{Extended Euler}
\(
a^b \equiv \begin{cases}
 a^{(b \mod{\varphi(m)}) + \varphi(m)}& \text{if } (a, m) \neq 1 \land b \geq \varphi(m) \\
 a^{b \mod{\varphi(m)}} & \text{otherwise}
\end{cases}
\pmod{m}
\)

\subsubsection{Pentagonal Number Theorem}
\(
\prod _{n=1}^{\infty }\left(1-x^{n}\right)=\sum _{k=-\infty }^{\infty }\left(-1\right)^{k}x^{k\left(3k-1\right)/2}=
\left(\sum p(n) x^n\right)^{-1}
\)
